ReactorModel/Objects/Reactor/Theorems/Finite.lean
@@ -1,5 +1,12 @@
 import ReactorModel.Objects.Reactor.Finite
+import ReactorModel.Objects.Reactor.Theorems.Hierarchical
 
-theorem Reactor.mem_ids_iff [Hierarchical α] [Finite α] {rtr : α} {i} : 
-    (i ∈ Finite.ids rtr cpt) ↔ (∃ o, rtr[cpt][i] = some o) := by
+namespace Reactor
+
+variable [Hierarchical α] [Finite α] {rtr rtr₁ rtr₂ : α}
+
+theorem mem_ids_iff : (i ∈ Finite.ids rtr cpt) ↔ (∃ o, rtr[cpt][i] = some o) := by
   simp [Finite.ids, ←Partial.mem_def, Partial.mem_iff]
+
+def equiv_card_eq (e : rtr₁ ≈ rtr₂) (cpt : Component) : rtr₁#cpt = rtr₂#cpt := by
+  simp only [Finite.card, Equivalent.ids_eq e]
