ReactorModel/Execution/Theorems.lean
@@ -3,9 +3,13 @@ import ReactorModel.Execution.Theorems.Grouped.Instantaneous
 import ReactorModel.Execution.Theorems.Grouped.Steps
 import ReactorModel.Execution.Theorems.Grouped.Tail
 import ReactorModel.Execution.Theorems.Step.Apply
+import ReactorModel.Execution.Theorems.Step.Basic
 import ReactorModel.Execution.Theorems.Step.Exec
 import ReactorModel.Execution.Theorems.Step.Skip
 import ReactorModel.Execution.Theorems.Step.Time
+import ReactorModel.Execution.Theorems.Variability.Basic
+import ReactorModel.Execution.Theorems.Variability.LoopModel
+import ReactorModel.Execution.Theorems.Variability.Weak
 import ReactorModel.Execution.Theorems.Dependency
 import ReactorModel.Execution.Theorems.Execution
 import ReactorModel.Execution.Theorems.Progress
