ReactorModel/Execution/Theorems/Execution.lean
@@ -11,7 +11,10 @@ theorem deterministic
     (e₁ : Execution s s₁) (e₂ : Execution s s₂) (ht : s₁.tag = s₂.tag)
     (hp : s₁.progress = s₂.progress) : s₁ = s₂ :=
   if h : s.Nontrivial
-  then (e₁.to_grouped h).deterministic h ht hp (e₂.to_grouped h)
+  then e₁.toGrouped.deterministic h ht hp e₂.toGrouped
   else e₁.trivial_deterministic h e₂ ht
 
-end Execution
+-- Property (1) on page 10 of https://www.informatik.uni-bremen.de/agbs/jp/papers/trs_script.pdf.
+theorem tag_le {s₁ s₂ : State α} : (Execution s₁ s₂) → s₁.tag ≤ s₂.tag
+  | .refl        => le_refl _
+  | .trans e₁ e₂ => e₁.tag_le.trans e₂.tag_le
