ReactorModel/Execution/Theorems/Variability/Weak.lean
@@ -1,6 +1,7 @@
 import ReactorModel.Execution.Theorems.Step.Basic
 import ReactorModel.Execution.Theorems.State
-import ReactorModel.Execution.Theorems.Monotonicity
+import ReactorModel.Execution.Theorems.Grouped.Basic
+import ReactorModel.Objects.Reactor.Theorems.Finite
 
 open Classical Reactor
 
@@ -20,49 +21,10 @@ def WeakFiniteVariability (α) [Hierarchical α] : Prop :=
 
 theorem weakly_finitely_variable [Proper α] [fin : Reactor.Finite α] : WeakFiniteVariability α := by
   intros t m s₁
-  let rcnCount := (Finite.fin s₁.rtr .rcn).toFinset.card
-  let maxTimeSteps := m - s₁.tag.microstep
-  -- Bound on the execution length:
-  -- reaction steps, time step, ..., reaction steps, time step, reaction steps
-  -- |____________ maxTimeSteps * (rcnCount + 1) _____________| + rcnCount
-  exists maxTimeSteps * (rcnCount + 1) + rcnCount
+  exists (m - s₁.tag.microstep) * (s₁.rtr#.rcn + 1) + (s₁.rtr#.rcn + 1)
   intro s₂ e ht₁ hm
-  induction e generalizing m <;> simp only [length, Nat.zero_le]
-  case trans s₂ s₃ e stp ih =>
-    change e.length < maxTimeSteps * (rcnCount + 1) + rcnCount
-    -- 1. We can somewhat easily establish s₁.time = s₂.time = s₃.time
-    have ht₂ : s₂.tag.time = t := sorry
-    have ht₃ : s₃.tag.time = t := sorry
-    have hm₃ : s₃.tag.microstep ≤ m := sorry -- by hm and ht₃
-    -- Depending on whether the final step is a time or a reaction step, we get different values
-    -- for `s₂.tag.microstep`.
-    cases stp
-    case time stp =>
-      have hm₂ : s₂.tag.microstep < s₃.tag.microstep := sorry -- by stp.tag_lt and ht₂, ht₃
-      have hm₂' := lt_of_lt_of_le hm₂ hm₃
-      specialize ih (m - 1) sorry -- by hm₂'
-      simp only [maxTimeSteps]
-      cases m
-      case zero => contradiction
-      case succ m =>
-        have hm₁ : s₁.tag.microstep < m := sorry -- by hm₂ and e
-        simp_all only [Nat.add_one_sub_one, gt_iff_lt]
-        suffices h : (m - s₁.tag.microstep) * (rcnCount + 1) + rcnCount < (m + 1 - s₁.tag.microstep) * (rcnCount + 1) + rcnCount by omega
-        simp_all only [Nat.add_lt_add_iff_right, Nat.zero_lt_succ, Nat.mul_lt_mul_right]
-        omega
-    -- TODO: These two cases should be analogous.
-    case skip stp =>
-      have hm₂ : s₂.tag.microstep = s₃.tag.microstep := by rw [stp.preserves_tag]
-      have hm₂' := hm₂ ▸ hm₃
-      specialize ih m sorry -- by hm₂'
-      simp [maxTimeSteps]
-      sorry -- PROBLEM: For this approach to work we'd need something like strong induction on
-            --          execution traces, so it's probably easier to take the grouped execution
-            --          approach instead.
-    case exec => sorry
-
-    -- 2. The number of time-steps taken from s₁ to s₃ is bounded by m - s₁.tag.microstep.
-    --    Thus, the length of e is also bounded by m - s₁.tag.microstep.
-    --    The number of steps that can be taken in an execution which takes at most N time steps
-    --    is bounded by N * (#rcns + 1) + #rcns.
-    --    TODO: Does our grouping theorem help with this?
+  let g := e.toGrouped
+  rw [e.toGrouped_length, Grouped.length]
+  apply Nat.add_le_add ?_ (equiv_card_eq g.steps.equiv _ ▸ g.tail.length_le)
+  suffices h : g.steps.steps = m - s₁.tag.microstep by exact h ▸ g.steps.length_le
+  sorry
